AP/AP/King.lean
@@ -5,9 +5,6 @@ namespace AP.King
 def state₀ : State :=
   initState 1 0
 
-def interior₁ : Set' PointZ :=
-  (0 : PointZ).nbhd Box.offset
-
 def dKingOp₂ : DStrat := .mk # λ s => List.head? # do
   let p ← Box.interior.toList
   guard # p ≠ s.aPos ∧ p ∉ s.taken
@@ -21,7 +18,93 @@ def dKingOp : DStrat := .mk' # λ s =>
   | none => dKingOp₁.f s
   | some p => p
 
+
 -----
+
+end King
+
+theorem AState.aPos_dist_le_of_tr {s s' p} [hs : AState s]
+(h : sys.tr s p = some s') : s'.aPos.dist s.aPos ≤ s.pw := by
+  simp [hs.tr_eq_some_iff] at h; grind
+
+theorem State.aPos_dist_le_of_simulate_two {s r f} [hs : sys.WF s]
+(h : sys.simulate f s 2 = r) : r.1.aPos.dist s.aPos ≤ s.pw := by
+  rcases r with ⟨s₂, r⟩; dsimp
+  simp [System.simulate] at h
+  split at h; simp at h; simp [←h]
+  nm x s₁ h₁
+  replace hs := s.aState_or_dState
+  rcases hs with hs | hs
+  · have hs₁ := DState.of_tr h₁
+    have h₂ := hs.aPos_dist_le_of_tr h₁
+    split at h
+    · nm x h₃; clear x
+      simp at h; simpa [←h]
+    nm x s₂ h₃; clear x
+    simp at h
+    rcases h with ⟨rfl, rfl⟩
+    rwa [DState.aPos_eq_of_tr h₃]
+  · have hs₁ := AState.of_tr h₁
+    have h₂ := hs.aPos_eq_of_tr h₁
+    split at h
+    · nm x h₃; clear x
+      simp at h
+      rcases h with ⟨rfl, rfl⟩
+      simp [h₂]
+    nm x s₂ h₃; clear x
+    simp at h
+    rcases h with ⟨rfl, rfl⟩
+    rw [←h₂]
+    rw [←pw_eq_of_tr h₁]
+    exact AState.aPos_dist_le_of_tr h₃
+
+theorem State.aPos_dist_le_of_simulate_mul_two {s r f n} [hs : sys.WF s]
+(h : sys.simulate f s (n * 2) = r) : r.1.aPos.dist s.aPos ≤ s.pw * n := by
+  subst r
+  induction n
+  · simp
+  nm n ih
+  simp [Nat.add_one_mul, sys.simulate_add]
+  generalize hr : sys.simulate f s (n * 2) = r at ih ⊢
+  rcases r with ⟨s₁, r⟩
+  dsimp at ih ⊢
+  generalize hr₁ : sys.simulate f s₁ 2 = r₁
+  rcases r₁ with ⟨s₃, r₁⟩
+  dsimp
+  split_ifs with h₁
+  rotate_left; grind
+  subst h₁
+  simp
+  have h₁ := sys.reachable_of_simulate_eq hr
+  have hs₁ := sys.wf_of_reachable h₁
+  suffices h : s₃.aPos.dist s₁.aPos ≤ s.pw
+  · suffices : s₃.aPos.dist s.aPos ≤ s₃.aPos.dist s₁.aPos + s₁.aPos.dist s.aPos; grind
+    apply Point.triangle
+  simp [←pw_eq_of_reachable h₁]
+  exact aPos_dist_le_of_simulate_two (r := ⟨s₃, r₁⟩) hr₁
+
+-- theorem State.aPos_distle_of_simulate_le {s f k n r₁ r₂} [hs : sys.WF s]
+-- (h₁ : sys.simulate f s k = r₁) (h₂ : sys.simulate f s n = r₂) (h₃ : k ≤ n) :
+-- r₁.1.aPos.dist s.aPos ≤ r₂.1.aPos.dist s.aPos := by
+--   obtain ⟨n, rfl⟩ := Nat.exists_eq_add_of_le h₃; clear h₃
+--   induction n generalizing r₂
+--   · simp at h₂; subst h₁ h₂; rfl
+--   nm n ih
+--   rw [←add_assoc, System.simulate_add] at h₂
+--   generalize hr : sys.simulate f s (k + n) = r at h₂
+--   rcases r with ⟨s₁, r⟩
+--   specialize ih hr
+--   simp at h₂
+--   split_ifs at h₂ with h₃
+--   rotate_left
+--   · subst h₂; simpa
+--   subst h₃
+--   rcases r₂ with ⟨s₂, r₂⟩
+--   simp at h₂ ⊢ ih
+
+-- #check 0 #exit
+
+namespace King
 
 @[simp]
 instance : dKingOp₂.WF := by
@@ -52,8 +135,29 @@ instance : dKingOp.WF := by
     simp; tauto
 
 @[simp]
-instance : sys.WF state₀ := by
+instance : DState state₀ := by
   unfold state₀; infer_instance
 
+@[simp] theorem pw_state₀ : state₀.pw = 1 := rfl
+@[simp] theorem aPos_state₀ : state₀.aPos = 0 := rfl
+
+-- #check 0 #exit
+
 theorem dWins_dKingOp {a : AStrat} [ha : a.WF] : state₀.dWins ⟨a, dKingOp⟩ := by
+  let f d n := sys.simulate (Strat.f ⟨a, d⟩) state₀ n
+  generalize hr : f dKingOp 200 = r
+  rcases r with ⟨s₁, n⟩
+  by_cases hn : n ≠ 0
+  · use 200; simpa [f, hr]
+  push_neg at hn; subst hn
+  have hs₁ := DState.of_simulate_mul_two_eq_full (n := 100) hr
+  
+  have h₁ : ∀ k ≤ 200, (f dKingOp k).1.aPos.dist 0 ≤ 100
+  ·
+    intro k hk
+    generalize hr₁ : f dKingOp k = r₁
+    have h₁ := State.aPos_dist_le_of_simulate_mul_two (n := 100) hr
+    simp at h₁
+    sorry
+  
   sorry
